chore: add cycle breaking heuristic for k-induction
This allows k-induction to bail out faster in the case of proving
safety properties on cycles in the FSM.

SSA/Experimental/Bits/Fast/ReflectVerif.lean
@@ -538,6 +538,10 @@ def Vars.castShift {n m : Nat} (v : Vars σ ι n) (hnm : n ≤ m) : Vars σ ι m
   | .state s => .state s
   | .inputs is => .inputs (is.castShift hnm)
 
+@[simp]
+theorem Vars.castLe_state {n m : Nat} (s : σ) (hnm : n ≤ m) :
+   (Vars.state s : Vars σ ι n).castLe hnm = Vars.state s := by rfl
+
 /-- casting to the same width equals vars-/
 @[simp]
 theorem Vars.castLe_eq_self {α : Type _} {n : Nat} (v : Vars α σ n) (h : n ≤ n) :
@@ -924,6 +928,17 @@ def mkCarryWith0Circuit {arity : Type _}
     { f : p.α → Circuit (Vars p.α arity 0) //
       ∀ (a : p.α), Circuit.Equiv (f a) (mkCarryWithCircuit p 0 a) } :=
   ⟨mkCarryWithCircuit p 0, by simp⟩
+
+@[simp]
+theorem eval_mkCarryWith0Circuit_eq {arity : Type _}
+    [DecidableEq arity]
+    [Fintype arity]
+    [Hashable arity]
+    (p : FSM arity) (s : p.α)
+    (envBool : Vars p.α arity 0 → Bool) :
+  ((mkCarryWith0Circuit p).val s).eval envBool = envBool (.state s) := by
+  simp only [mkCarryWith0Circuit, mkCarryWithCircuit, Circuit.eval, Circuit.var, Vars.state]
+  rcases h : envBool (Vars.state s) <;> simp [h]
 
 /--
 make the CarryWith circuit for step (n+1), incrementally,
@@ -1398,6 +1413,245 @@ def mkIndHypCircuit {arity : Type _}
   mkUnsatImpliesCircuit
     ((mkEvalWithNCircuit p n).map (fun vs => vs.castLe (by omega)))
     (mkEvalWithCircuit p (n + 1))
+
+/-- Make a circuit that checks if two states are equal. -/
+def mkStateEqCircuit
+  {arity : Type _} {i : Nat}
+  [DecidableEq arity] [Fintype arity] [Hashable arity]
+  (p : FSM arity) (s t : p.α → Circuit (Vars p.α arity i)) : Circuit (Vars p.α arity i) :=
+  Circuit.bigOr <| FinEnum.toList p.α |>.map fun a => (s a) ^^^ (t a)
+
+
+/-- if the state circuit is false, then the states are equal under all evaluations. -/
+theorem mkStateEqCircuit_eq_zero_iff {arity : Type _} {i : Nat}
+  [DecidableEq arity] [Fintype arity] [Hashable arity]
+  (p : FSM arity) (s t : p.α → Circuit (Vars p.α arity i)) :
+  (∀ envBool, (mkStateEqCircuit p s t).eval envBool = false) ↔
+  (∀ (a : p.α) (envBool : Vars p.α arity i → Bool), (s a).eval envBool = (t a).eval envBool) := by
+  simp [mkStateEqCircuit, Circuit.eval_bigOr_eq_false_iff]
+  constructor
+  · intros h a envBool
+    apply h
+  · intros h envBool a
+    apply h
+
+
+/-- Make a circuit that checks if two states are disequal. -/
+def mkStateNeqCircuit
+  {arity : Type _} {i : Nat}
+  [DecidableEq arity] [Fintype arity] [Hashable arity]
+  (p : FSM arity) (s t : p.α → Circuit (Vars p.α arity i)) : Circuit (Vars p.α arity i) :=
+  Circuit.bigAnd <| FinEnum.toList p.α |>.map fun a => ~~~ (s a) ^^^ (t a)
+
+
+/-- if the state circuit is false, then the states are equal under all evaluations. -/
+@[simp]
+theorem mkStateNeqCircuit_eq_false_iff {arity : Type _} {i : Nat}
+  [DecidableEq arity] [Fintype arity] [Hashable arity]
+  (p : FSM arity) (s t : p.α → Circuit (Vars p.α arity i)) :
+  (∀ envBool, (mkStateNeqCircuit p s t).eval envBool = false) ↔
+  (∀ (envBool : Vars p.α arity i → Bool), ∃ (a : p.α), (s a).eval envBool ≠ (t a).eval envBool) := by
+  simp [mkStateNeqCircuit, Circuit.eval_bigAnd_eq_false_iff]
+
+/-- if the stateNeq circuit is false at a current environment,
+then the states disagree at this environment. -/
+@[simp]
+theorem mkStateNeqCircuit_eq_false_iff₂  {arity : Type _} {i : Nat}
+  [DecidableEq arity] [Fintype arity] [Hashable arity]
+  (p : FSM arity) (s t : p.α → Circuit (Vars p.α arity i))
+  (envBool : Vars p.α arity i → Bool) :
+  ((mkStateNeqCircuit p s t).eval envBool = false) ↔
+  ∃ (a : p.α), (s a).eval envBool ≠ (t a).eval envBool := by
+  simp [mkStateNeqCircuit, Circuit.eval_bigAnd_eq_false_iff]
+
+/--
+make the circuit that witnesses that the states are unique *after* taking 'i+1' inputs.
+We take 'i+1' so that we take at least one input.
+This circuit produces false iff...
+-/
+def mkUniqueStateCircuitAux {arity : Type _}
+  [DecidableEq arity] [Fintype arity] [Hashable arity]
+  (p : FSM arity) (i : Nat) : Circuit (Vars p.α arity (i+1)) :=
+   let ins := mkCarryWith0Circuit p |>.val
+   let outs := mkCarryWithCircuit p (i+1)
+   (mkStateNeqCircuit p outs (fun s => (ins s).map  (fun v => v.castLe (by omega))))
+
+
+@[simp]
+theorem mkUniqueStateCircuitAux_eq_false_iff {arity : Type _}
+  [DecidableEq arity] [Fintype arity] [Hashable arity]
+  (p : FSM arity) (i : Nat) :
+  (∀ (envBool : Vars p.α arity (i + 1) → Bool), (mkUniqueStateCircuitAux p i).eval envBool = false) ↔
+  (∀ (envBitstream : arity → BitStream) (state : p.α → Bool) , ¬ (p.carryWith state envBitstream (i + 1) = state)) := by
+  simp [mkUniqueStateCircuitAux, mkStateEqCircuit_eq_zero_iff]
+  constructor
+  · intros h envBitstream state
+    let envBool := envBool_of_envBitstream_of_state envBitstream state i
+    specialize h envBool
+    apply Function.ne_iff.mpr
+    obtain ⟨a, ha⟩ := h
+    exists a
+    simp only [mkCarryWith0Circuit] at ha
+    simp only [Circuit.eval_map, Circuit.eval, ↓reduceIte, Vars.castLe_state] at ha
+    rw [eval_mkCarryWithCircuit_eq_carryWith (envBitstream := envBitstream)] at ha
+    · apply ha
+    · simp [envBool]
+  · intros h envBool
+    let envBitstream := Bitstream_of_envBool envBool
+    let state := fun s => envBool (.state s)
+    specialize h envBitstream state
+    have := Function.ne_iff.mp h
+    obtain ⟨a, ha⟩ := this
+    exists a
+    rw [Circuit.eval_map, eval_mkCarryWith0Circuit_eq]
+    rw [eval_mkCarryWithCircuit_eq_carryWith (envBitstream := envBitstream)]
+    · simp only [Vars.castLe_state]
+      apply ha
+    · simp [envBitstream]
+
+
+@[simp]
+theorem mkUniqueStateCircuitAux_eq_false_iff_of_EnvOutRelated {arity : Type _}
+    [DecidableEq arity] [Fintype arity] [Hashable arity]
+    (p : FSM arity) (i : Nat)
+    (envBool : Vars p.α arity (i + 1) → Bool)
+    (envBitstream : arity → BitStream)
+    (hEnvBitstream : EnvOutRelated envBool envBitstream) :
+    (((mkUniqueStateCircuitAux p i).eval envBool = false) ↔
+      ¬ (p.carryWith (fun s => envBool (.state s)) envBitstream (i + 1) = (fun s => envBool (.state s)))) := by
+  constructor
+  · intros h
+    let state := fun s => envBool (.state s)
+    apply Function.ne_iff.mpr
+    simp at h
+    rw [mkUniqueStateCircuitAux] at h
+    simp at h
+    obtain ⟨a, ha⟩ := h
+    exists a
+    rw [eval_mkCarryWithCircuit_eq_carryWith] at ha
+    rw [Circuit.eval_map] at ha
+    rw [eval_mkCarryWith0Circuit_eq] at ha
+    simp only [Circuit.eval_map, Circuit.eval, ↓reduceIte, Vars.castLe_state] at ha
+    · apply ha
+    · apply hEnvBitstream
+  · intros h
+    have := Function.ne_iff.mp h
+    obtain ⟨a, ha⟩ := this
+    rw [mkUniqueStateCircuitAux]
+    simp
+    exists a
+    rw [Circuit.eval_map, eval_mkCarryWith0Circuit_eq]
+    rw [eval_mkCarryWithCircuit_eq_carryWith (envBitstream := envBitstream)]
+    · simp only [Vars.castLe_state]
+      apply ha
+    · apply hEnvBitstream
+
+/--
+make the circuit that witnesses that the states are unique *after* taking 'i+1' inputs.
+This circuit produce false iff there are two states that are equal in [1..i+1] inputs
+-/
+def mkUniqueStatesCircuit {arity : Type _}
+  [DecidableEq arity] [Fintype arity] [Hashable arity]
+  (p : FSM arity) (i : Nat) : Circuit (Vars p.α arity (i+1)) :=
+  let xs := List.range (i + 1) |>.attach
+  Circuit.bigOr <| xs.map fun j =>
+    (mkUniqueStateCircuitAux p j.val).map (fun v =>
+      v.castLe (by have := j.property; simp at this; omega))
+
+
+@[simp]
+theorem mkUniqueStatesCircuit_eq_false_iff_of_EnvOutRelated {arity : Type _}
+  [DecidableEq arity] [Fintype arity] [Hashable arity]
+  (p : FSM arity) (i : Nat)
+  (envBool : Vars p.α arity (i + 1) → Bool)
+  (envBitstream : arity → BitStream)
+  (hEnvBitstream : EnvOutRelated envBool envBitstream) :
+  ((mkUniqueStatesCircuit p i).eval envBool = false) ↔
+  (∀(j : Nat), j < i + 1 →
+    ¬ (p.carryWith (fun s => envBool (.state s)) envBitstream (j + 1) =
+        (fun s => envBool (.state s)))) := by
+  simp [mkUniqueStatesCircuit, Circuit.eval_bigOr_eq_false_iff]
+  constructor
+  · intros h j hj
+    specialize h _ j hj rfl
+    rw [Circuit.eval_map] at h
+    rw [mkUniqueStateCircuitAux_eq_false_iff_of_EnvOutRelated
+      (envBitstream := envBitstream)] at h
+    · simp only [Vars.castLe_state] at h
+      apply h
+    · constructor
+      intros x k hk
+      apply hEnvBitstream.envBool_inputs_mk_eq_envBitStream
+  · intros h c
+    intros j hj
+    intros hc
+    subst hc
+    rw [Circuit.eval_map]
+    rw [mkUniqueStateCircuitAux_eq_false_iff_of_EnvOutRelated
+      (envBitstream := envBitstream)]
+    · apply h j hj
+    · constructor
+      intros x k hk
+      apply hEnvBitstream.envBool_inputs_mk_eq_envBitStream
+
+/-- mkUniqueStatesCircuit is false iff we don't have a repeatin state. -/
+@[simp]
+theorem mkUniqueStatesCircuit_eq_false_iff {arity : Type _}
+  [DecidableEq arity] [Fintype arity] [Hashable arity]
+  (p : FSM arity) (i : Nat) :
+  (∀ (envBool : Vars p.α arity (i + 1) → Bool), (mkUniqueStatesCircuit p i).eval envBool = false) ↔
+  (∀ (envBitstream : arity → BitStream) (state : p.α → Bool) (j : Nat),
+    j < i +1 → ¬ (p.carryWith state envBitstream (j + 1) = state)) := by
+  simp [mkUniqueStatesCircuit, Circuit.eval_bigOr_eq_false_iff]
+  constructor
+  · intros h envBitstream state
+    let envBool := envBool_of_envBitstream_of_state envBitstream state i
+    specialize h envBool
+    intros j hj
+    specialize h _ j hj rfl
+    rw [Circuit.eval_map] at h
+    rw [mkUniqueStateCircuitAux_eq_false_iff_of_EnvOutRelated
+      (envBitstream := envBitstream)] at h
+    · simp only [Vars.castLe_state, envBool_of_envBitstream_of_state_eq₁, envBool] at h
+      apply h
+    · constructor
+      intros x k hk
+      rfl -- TODO: don't exploit 'rfl' here.
+  · intros h envBool
+    let envBitstream := Bitstream_of_envBool envBool
+    let state := fun s => envBool (.state s)
+    specialize h envBitstream state
+    intros c j hj hc
+    subst hc
+    rw [Circuit.eval_map]
+    rw [mkUniqueStateCircuitAux_eq_false_iff_of_EnvOutRelated
+      (envBitstream := envBitstream)]
+    · apply h j hj
+    · constructor
+      intros x k hk
+      simp only [Bitstream_of_envBool, envBitstream]
+      simp only [show k < i + 1 by omega, ↓reduceDIte, envBitstream]
+      rfl
+
+/--
+make the circuit that witnesses that the states are unique *after* taking 'i+1' inputs.
+This circuit produce false iff there are two states that are equal in [1..i+1] inputs
+-/
+def mkAllPairsUniqueStatesCircuit {arity : Type _}
+  [DecidableEq arity] [Fintype arity] [Hashable arity]
+  (p : FSM arity) (n : Nat) : Circuit (Vars p.α arity (n+1)) :=
+  let xs := List.range (n + 1) |>.attach
+
+  Circuit.bigOr <| xs.flatMap fun i =>
+    let ys := List.range i.val |>.attach
+    ys.map fun j =>
+     let si : p.α → Circuit (Vars p.α arity (n+1)) := fun s =>
+       (mkCarryWithCircuit p (i.val +1) s).map (fun v =>
+         v.castLe (by have := i.property; simp at this; omega))
+     let sj : p.α → Circuit (Vars p.α arity (n+1)) := fun s =>
+       (mkCarryWithCircuit p (j.val +1) s).map (fun v =>
+         v.castLe (by have := j.property; simp at this; have := i.property; simp at this; omega))
+     (mkStateNeqCircuit (i := (n+1)) p si sj)
 
 
 /-- induction hyp circuit. -/
